theories/int_ptr_cast.v
@@ -1,0 +1,388 @@
+Require Export refframe.module.
+Require Import refframe.trefines.
+Require Import refframe.filter.
+Require Import refframe.product.
+Require Import refframe.seq_product.
+Require Import refframe.link.
+Require Import refframe.proof_techniques.
+Require Import refframe.prepost.
+Require Import refframe.imp.
+Require Import refframe.asm.
+Require Import refframe.itree.
+Require Import refframe.imp_to_asm.
+
+Local Open Scope Z_scope.
+
+Definition int_to_ptr_asm : gmap Z asm_instr :=
+  (* cast_int_to_ptr *)
+  <[ 400 := [
+        (* ret *)
+        WriteReg "PC" (λ rs, rs !!! "R30")
+    ] ]> $
+  (* cast_ptr_to_int *)
+  <[ 404 := [
+        (* ret *)
+        WriteReg "PC" (λ rs, rs !!! "R30")
+    ] ]> $ ∅.
+
+Definition int_to_ptr_itree : itree (moduleE imp_event (gmap prov Z)) unit :=
+  ITree.forever (
+      f ← TExist string;;;
+      vs ← TExist (list val);;;
+      h ← TExist (heap_state);;;
+      TVis (Incoming, EICall f vs h);;;;
+      if bool_decide (f = "cast_int_to_ptr") then
+        z ← TAll Z;;;
+        TAssume (vs = [ValNum z]);;;;
+        l ← TAll loc;;;
+        ps ← TGet;;;
+        TAssume (ps !! l.1 = Some (z - l.2));;;;
+        TVis (Outgoing, EIReturn (ValLoc l) h)
+      else if bool_decide (f = "cast_ptr_to_int") then
+        l ← TAll loc;;;
+        TAssume (vs = [ValLoc l]);;;;
+        z ← TExist Z;;;
+        ps ← TGet;;;
+        let ps' := <[l.1 := (default z (ps !! l.1))]> ps in
+        TPut ps';;;;
+        TVis (Outgoing, EIReturn (ValNum (ps' !!! l.1 + l.2)) h)
+      else
+        TNb).
+
+Local Ltac go :=
+  clear_itree.
+Local Ltac go_s :=
+  tstep_s; go.
+Local Ltac go_i :=
+  tstep_i; go.
+
+Lemma int_to_ptr_asm_refines_itree :
+  trefines (MS asm_module (initial_asm_state int_to_ptr_asm))
+           (MS (imp_to_asm (dom _ int_to_ptr_asm) ({[ "cast_int_to_ptr"; "cast_ptr_to_int" ]})
+                           (<["cast_int_to_ptr" := 400]> $ <["cast_ptr_to_int" := 404]> $ ∅)
+                           (mod_itree imp_event (gmap prov Z)))
+               (initial_imp_to_asm_state (mod_itree _ _) (int_to_ptr_itree, ∅))).
+Proof.
+  apply: tsim_implies_trefines => n0 /=.
+  unshelve eapply tsim_remember. { simpl. exact (λ _ σa '(σf, (t, ps), (pp, σi2a, P)),
+    t ≈ int_to_ptr_itree ∧
+    σa.(asm_cur_instr) = None ∧
+    σa.(asm_instrs) = int_to_ptr_asm ∧
+    σi2a.(i2a_calls) = [] ∧
+    σf = SMFilter ∧
+    pp = PPOutside ∧
+    (P ⊢ [∗ map] p↦z∈ps, i2a_heap_shared p z)). }
+  { split!. by rewrite big_sepM_empty. } { done. }
+  move => n _ Hloop [????] [[?[? ps]][[??]?]] ?. destruct_all?; simplify_eq/=.
+  tstep_i => ????? Hi. tstep_s. split!. tstep_s => *. case_match => /= *. 2: congruence.
+  tstep_s. rewrite -/int_to_ptr_itree. go. go_s. eexists _. go. go_s. eexists _. go. go_s. eexists _. go.
+  go_s. split!. go.
+  revert select (_ ⊢ _) => HP.
+  revert select (imp_to_asm_args _ _ _) => -[?[?[??]]].
+  revert select (_ ∉ dom _ _) => /not_elem_of_dom?.
+  unfold int_to_ptr_asm in Hi. (repeat case_bool_decide); simplify_map_eq.
+  - tstep_i. split; [by simplify_map_eq'|].
+    go_s => ?. go.
+    go_s => ?. go.
+    go_s => ?. go.
+    go_s. go_s => ?. go.
+    iSatStart. iIntros!.
+    iDestruct (big_sepL2_cons_inv_l with "[$]") as (???) "[% ?]".
+    iDestruct (big_sepL2_nil_inv_l with "[$]") as %?. simplify_eq/=.
+    decompose_Forall_hyps.
+    iDestruct (HP with "[$]") as "HP".
+    iDestruct (big_sepM_lookup with "HP") as "#?"; [done|].
+    iSatStop.
+    tstep_i => ??. simplify_map_eq'.
+    go_s. go_s. split!. { by simplify_map_eq'. }
+    1: { unfold imp_to_asm_ret; split!; simplify_map_eq'; split!.
+         - by apply map_list_included_insert.
+         - apply map_preserved_insert_r_not_in; [|done]. compute_done.
+    }
+    { apply map_scramble_insert_r_in; [compute_done|done]. }
+    { iSatMono. simplify_map_eq'. iIntros!. iFrame. iSplitL; [iAccu|]. iSplit!; [|done]. lia. }
+    apply Hloop; [done|].
+    split!.
+  - tstep_i. split; [by simplify_map_eq'|].
+    go_s => l. go.
+    go_s => ?. go.
+    iSatStart. iIntros!.
+    iDestruct (big_sepL2_cons_inv_l with "[$]") as (???) "[#[%z ?] ?]".
+    iDestruct (big_sepL2_nil_inv_l with "[$]") as %?. simplify_eq/=.
+    iDestruct!.
+    iDestruct (HP with "[$]") as "HP".
+    iDestruct (i2a_heap_shared_lookup with "[$] [$]") as %?. setoid_subst.
+    decompose_Forall_hyps.
+    iAssert ⌜z = default z (ps !! l.1)⌝%I as %Hz.
+    { destruct (ps !! l.1) as [z'|] eqn:Hp => //=.
+      iDestruct (big_sepM_lookup with "HP") as "?"; [done|].
+      iAssert ⌜z = z'⌝%I as %?; [|done].
+      by iApply i2a_heap_shared_ag. }
+    iSatStop.
+    go_s. eexists z. go.
+    go_s. go_s. go_s.
+    tstep_i => ??. simplify_map_eq'.
+    go_s. split!. { by simplify_map_eq'. }
+    1: { unfold imp_to_asm_ret; split!; simplify_map_eq'; split!.
+         - by apply map_list_included_insert.
+         - apply map_preserved_insert_r_not_in; [|done]. compute_done.
+    }
+    { apply map_scramble_insert_r_in; [compute_done|done]. }
+    { iSatMono. simplify_map_eq'. iFrame. iSplitL; [by iStopProof|].
+      rewrite -Hz. done.
+    }
+    apply Hloop; [done|].
+    split!.
+    iIntros "[#? #?]". rewrite -Hz.
+    by iApply big_sepM_insert_2.
+Qed.
+
+Definition main_imp : fndef := {|
+  fd_args := [];
+  fd_body := LetE "l" (Alloc (Val 1)) $
+             LetE "_" (Store (Var "l") (Val 1)) $
+             LetE "z" (imp.Call "cast_ptr_to_int" [(Var "l")]) $
+             LetE "z'" (BinOp (BinOp (Var "z") AddOp (Val (-1))) AddOp (Val 1)) $
+             LetE "l'" (imp.Call "cast_int_to_ptr" [(Var "z")]) $
+             LetE "r" (Load (Var "l'")) $
+             LetE "_" (Free (Var "l")) $
+             imp.Call "exit" [(Var "r")];
+  fd_static := I
+|}.
+
+Definition main_imp_prog : gmap string fndef :=
+  <[ "main" := main_imp ]> ∅.
+
+Definition main_itree : itree (moduleE imp_event unit) unit :=
+  f ← TExist string;;;
+  vs ← TExist (list val);;;
+  h ← TExist (heap_state);;;
+  TVis (Incoming, EICall f vs h);;;;
+  TAssume (f = "main");;;;
+  TAssume (vs = []);;;;
+  h' ← TExist (heap_state);;;
+  TVis (Outgoing, EICall "exit" [ValNum 1] h');;;;
+  TUb.
+
+Lemma main_int_to_ptr_refines_itree :
+  trefines (MS (imp_prod (dom _ main_imp_prog) ({[ "cast_int_to_ptr"; "cast_ptr_to_int" ]})
+                         imp_module (mod_itree _ _))
+               (MLFNone, [], initial_imp_state main_imp_prog, (int_to_ptr_itree, ∅)))
+           (MS (mod_itree _ _) (main_itree, tt)).
+Proof.
+  apply: tsim_implies_trefines => n0 /=.
+  tstep_i => *. case_match; destruct_all?; simplify_eq.
+  go_s. eexists _. go. go_s. eexists _. go. go_s. eexists _. go.
+  go_s. split!. go.
+  go_s => ?. go. go_s => ?. go. simplify_eq. rewrite bool_decide_true; [|compute_done].
+  tstep_i. split! => ???? Hf ?. unfold main_imp_prog in Hf. simplify_map_eq.
+  tstep_i => l ?. split!.
+  tstep_i.
+  tstep_i. split. { apply heap_alive_alloc; [done|lia]. }
+  tstep_i. change ([Val (ValLoc l)]) with (Val <$> [ValLoc l]).
+  tstep_i. split. { move => *; simplify_map_eq. }
+  move => ????. rewrite bool_decide_false; [|compute_done]. rewrite bool_decide_true; [|compute_done].
+  move => *. destruct_all?. simplify_eq/=.
+  tstep_i. rewrite -/int_to_ptr_itree. go.
+  go_i => ?. go.
+  go_i => ?. go.
+  go_i => ?. go.
+  go_i => ?. go. simplify_eq/=.
+  go_i. eexists _. go.
+  go_i. split!. go.
+  go_i => z. go.
+  go_i. go_i. simplify_map_eq'.
+  go_i => *. go. destruct_all?; simplify_eq.
+  go_i. split!. move => *. simplify_eq.
+  go_i.
+  go_i.
+  go_i.
+  go_i. change ([Val (z + l.2)]) with (Val <$> [ValNum (z + l.2)]).
+  tstep_i. split. { move => *; simplify_map_eq. }
+  move => ????. rewrite bool_decide_false; [|compute_done]. rewrite bool_decide_true; [|compute_done].
+  move => *. destruct_all?. simplify_eq/=.
+  tstep_i. rewrite -/int_to_ptr_itree. go.
+  go_i => ?. go.
+  go_i => ?. go.
+  go_i => ?. go.
+  go_i => ?. go. simplify_eq/=.
+  go_i. eexists _. go.
+  go_i. split!. go.
+  go_i. eexists l. go.
+  go_i.
+  go_i. simplify_map_eq. split; [f_equal; lia|]. go.
+  go_i => *. go. destruct_all?; simplify_eq.
+  go_i. split!. move => *. simplify_eq.
+  go_i.
+  go_i. eexists _. split. { rewrite shift_loc_0. by simplify_map_eq. }
+  go_i.
+  go_i. split. { apply heap_alive_update. apply heap_alive_alloc; [done|lia]. }
+  go_i. change ([Val 1]) with (Val <$> [ValNum 1]).
+  go_i. split. { move => *; simplify_map_eq. }
+  move => ????. rewrite bool_decide_false; [|compute_done].
+  move => *. destruct_all?. simplify_eq/=.
+  go_s. eexists _. go.
+  go_s. split!. go.
+  go_s. done.
+Qed.
+
+Definition __NR_EXIT : Z := 93.
+
+Definition exit_asm : gmap Z asm_instr :=
+  (* exit *)
+  <[ 100 := [
+        WriteReg "R8" (λ rs, __NR_EXIT);
+        WriteReg "PC" (λ rs, rs !!! "PC" + 4)
+    ] ]> $
+  <[ 104 := [
+        Syscall false;
+        WriteReg "PC" (λ rs, rs !!! "PC" + 4)
+    ] ]> $
+  <[ 108 := [
+        (* loop *)
+        WriteReg "PC" (λ rs, rs !!! "PC")
+    ] ]> $ ∅.
+
+Definition exit_itree : itree (moduleE asm_event unit) unit :=
+  pc ← TExist _;;;
+  rs ← TExist _;;;
+  mem ← TExist _;;;
+  TVis (Incoming, EAJump pc rs mem);;;;
+  TAssume (pc = 100);;;;
+  TAssume (map_list_included syscall_arg_regs rs);;;;
+  args ← TExist _;;;
+  TAssert (length args = length syscall_arg_regs);;;;
+  TAssert (args !! 0%nat = Some (rs !!! "R0"));;;;
+  TAssert (args !! 8%nat = Some __NR_EXIT);;;;
+  TVis (Outgoing, EASyscallCall args);;;;
+  ret ← TExist _;;;
+  TVis (Incoming, EASyscallRet ret);;;;
+  TNb.
+
+Lemma exit_asm_refines_itree :
+  trefines (MS asm_module (initial_asm_state exit_asm))
+           (MS (mod_itree _ _) (exit_itree, tt)).
+Proof.
+  apply: tsim_implies_trefines => n0 /=.
+  go_i => ????? Hi.
+  go_s. eexists _. go.
+  go_s. eexists _. go.
+  go_s. eexists _. go.
+  go_s. split!. go.
+  go_s => ?. go.
+  go_s => ?. go.
+  unfold exit_asm in Hi. simplify_map_eq.
+  go_i. split. { apply: map_list_included_is_Some; [done|]. compute_done. }
+  go_i. split. { by simplify_map_eq. }
+  go_i => ??. simplify_map_eq'.
+  go_i.
+  go_s. eexists _. go.
+  go_s. split; [shelve|]. go.
+  go_s. split; [shelve|]. go.
+  go_s. split; [shelve|]. go.
+  go_s. split!. go.
+  go_i => ?.
+  go_s. eexists _. go.
+  go_s. split!. go.
+  go_i. split. { by simplify_map_eq. }
+  sort_map_insert. simplify_map_eq'.
+  unshelve eapply tsim_remember. { exact (λ _ '(AsmState i rs _ ins) _,
+      i = Some [] ∧ rs !! "PC" = Some 108 ∧ ins = exit_asm). }
+  { split!. by simplify_map_eq. } { done. }
+  move => ?? Hloop [????] ? ?. destruct_all?; simplify_eq.
+  go_i => ??. simplify_map_eq.
+  go_i. split. { by simplify_map_eq. }
+  apply Hloop; [done|]. split!. by simplify_map_eq'.
+  Unshelve.
+  - done.
+  - by simplify_map_eq'.
+  - by simplify_map_eq'.
+Qed.
+
+Definition top_level_itree : itree (moduleE asm_event unit) unit :=
+  pc ← TExist _;;;
+  rs ← TExist _;;;
+  mem ← TExist _;;;
+  TVis (Incoming, EAJump pc rs mem);;;;
+  TAssume (pc = 200);;;;
+  TAssume (map_list_included tmp_registers rs);;;;
+  TAssume (map_list_included saved_registers rs);;;;
+  TAssume (rs !!! "R30" ∉ ({[200; 400; 404]} : gset _));;;;
+  args ← TExist _;;;
+  TAssert (length args = length syscall_arg_regs);;;;
+  TAssert (args !! 0%nat = Some 1);;;;
+  TAssert (args !! 8%nat = Some __NR_EXIT);;;;
+  TVis (Outgoing, EASyscallCall args);;;;
+  ret ← TExist _;;;
+  TVis (Incoming, EASyscallRet ret);;;;
+  TNb.
+
+Lemma top_level_refines_itree :
+  trefines (MS (asm_prod {[200; 400; 404]} {[ 100; 104; 108 ]}
+                         (imp_to_asm {[200; 400; 404]} {[ "main" ; "cast_int_to_ptr"; "cast_ptr_to_int" ]}
+                                     (<[ "main" := 200 ]> $
+                                      <[ "cast_int_to_ptr" := 400 ]> $
+                                      <[ "cast_ptr_to_int" := 404 ]> $
+                                      <[ "exit" := 100 ]> $ ∅)
+                                     (mod_itree _ _)) (mod_itree _ _))
+               (MLFNone, None, initial_imp_to_asm_state (mod_itree _ _) (main_itree, tt), (exit_itree, tt)))
+           (MS (mod_itree _ _) (top_level_itree, tt)).
+Proof.
+  apply: tsim_implies_trefines => n0 /=.
+  go_i => ?????. case_match; destruct_all?; simplify_eq.
+  go_s. eexists _. go.
+  go_s. eexists _. go.
+  go_s. eexists _. go.
+  go_s. split!. go.
+  go_s => ?. go.
+  go_s => ?. go.
+  go_s => ?. go.
+  go_s => ?. go. simplify_eq/=.
+  rewrite bool_decide_true; [|compute_done].
+  go_i => ??. simplify_eq.
+  go_i. eexists true => /=. split; [done|]. eexists ∅, ∅, ∅.
+  split. { admit. }
+  eexists (regs !!! "R30"), "main", [], [].
+  split!. { unfold imp_to_asm_args. split!. apply lookup_lookup_total.
+            apply: (map_list_included_is_Some tmp_registers); [done|]. compute_done. }
+  { admit. }
+  go_i => ?. go.
+  go_i => ?. go.
+  go_i => ?. go.
+  go_i => ?. go. simplify_eq.
+  go_i. split!. go.
+  go_i. split!. go.
+  go_i => ?. go.
+  go_i.
+  go_i. move => *. destruct_all?; simplify_map_eq.
+  rewrite bool_decide_false; [|compute_done]. rewrite bool_decide_true; [|compute_done].
+  go_i => ?. go.
+  go_i => ?. go.
+  go_i => ?. go.
+  go_i => ?. go. simplify_eq.
+  go_i. split!. go.
+  go_i. split!. { admit. } go.
+  go_i => ?. go.
+  go_i => ?. go.
+  go_i => ?. go.
+  go_i => ?. go.
+  go_i => *. destruct_all?; simplify_eq. go.
+  go_s. eexists _. go.
+  go_s. split; [shelve|]. go.
+  go_s. split; [shelve|]. go.
+  go_s. split; [shelve|]. go.
+  go_s. split!. go.
+  go_i => *. case_match; destruct_all?; simplify_eq.
+  go_s. eexists _. go.
+  go_s. split!. go.
+  go_i => *. go.
+  go_i => *. go.
+  go_i => *. done.
+  Unshelve.
+  - admit.
+  - admit.
+  - done.
+  - iSatStart. iIntros!. iDestruct (big_sepL2_cons_inv_l with "[$]") as (????) "?". iSatStop. simplify_eq.
+    revert select (imp_to_asm_args _ _ _) => -[?[??]]. decompose_Forall_hyps. simplify_map_eq'. by f_equal.
+  - done.
+Admitted.
